Add doc comments to Models

ExistentialRules/Models/Cores.lean
@@ -1,887 +1,968 @@
 import ExistentialRules.Models.Basic
 
+/-!
+# Cores
+
+In this file, we define cores of fact sets. Namely, we define `FactSet.isWeakCore` and `FactSet.isStrongCore`.
+`FactSet`s that are models and cores are interesting since there are (intuitively speaking) the smallest possible models.
+Under certain condition, the chase is able to produce a core directly, which is very desirable since the result of the chase is also always a universal model.
+But this is discussed in other files. Here, we are only concerned with the definition of cores on `FactSet`s and some of their properties.
+-/
+
+/-!
+## Some Auxiliary Definitions and Theorems on Lists and Functions
+
+Before we can go into the actual definitions, we need a lot of machinery, mainly about functions to be able to state properties like injectivity and surjectivity possibly only about a list of set of elements and not the whole domain of the function.
+-/
+
 namespace List
 
-  theorem length_le_of_nodup_of_all_mem [DecidableEq α] (as bs : List α) (nodup : as.Nodup) (all_mem : ∀ e, e ∈ as -> e ∈ bs) : as.length ≤ bs.length := by
-    induction as generalizing bs with
-    | nil => simp
+/-!
+### Auxiliary Theorems on Lists
+-/
+
+/-- If a list is duplicate free and the sublist of another list, then the second list is at least as long as the first. -/
+theorem length_le_of_nodup_of_all_mem [DecidableEq α] (as bs : List α) (nodup : as.Nodup) (all_mem : ∀ e, e ∈ as -> e ∈ bs) : as.length ≤ bs.length := by
+  induction as generalizing bs with
+  | nil => simp
+  | cons a as ih =>
+    let bs_without_a := bs.erase a
+    simp only [nodup_cons] at nodup
+    specialize ih
+      bs_without_a
+      nodup.right
+      (by intro c c_mem; rw [List.mem_erase_of_ne]; apply all_mem; simp [c_mem]; intro contra; rw [contra] at c_mem; apply nodup.left; exact c_mem)
+    rw [List.length_erase_of_mem (by apply all_mem; simp)] at ih
+    rw [Nat.le_sub_one_iff_lt (by apply List.length_pos_of_mem; apply all_mem a; simp)] at ih
+    apply Nat.succ_le_of_lt
+    exact ih
+
+/-- If a list is duplicate free and the sublist of another list that has the same length, then both lists have exactly the same elements. -/
+theorem equiv_of_nodup_of_length_eq_of_all_mem [DecidableEq α] (as bs : List α) (nodup : as.Nodup) (eq_length : as.length = bs.length) (all_mem : ∀ e, e ∈ as -> e ∈ bs) : ∀ e, e ∈ as ↔ e ∈ bs := by
+  intro e
+  constructor
+  . apply all_mem
+  . intro mem_bs
+    induction as generalizing bs e with
+    | nil => cases bs; simp at mem_bs; simp at eq_length
     | cons a as ih =>
       let bs_without_a := bs.erase a
-      simp at nodup
+      simp only [nodup_cons] at nodup
       specialize ih
         bs_without_a
         nodup.right
+        (by rw [List.length_erase_of_mem, ← eq_length]; simp; apply all_mem; simp)
         (by intro c c_mem; rw [List.mem_erase_of_ne]; apply all_mem; simp [c_mem]; intro contra; rw [contra] at c_mem; apply nodup.left; exact c_mem)
-      rw [List.length_erase_of_mem (by apply all_mem; simp)] at ih
-      rw [Nat.le_sub_one_iff_lt (by apply List.length_pos_of_mem; apply all_mem a; simp)] at ih
-      apply Nat.succ_le_of_lt
-      exact ih
+      cases Decidable.em (e = a) with
+      | inl eq => simp [eq]
+      | inr neq =>
+        simp only [mem_cons]; apply Or.inr
+        apply ih
+        rw [List.mem_erase_of_ne]
+        exact mem_bs
+        exact neq
 
-  theorem equiv_of_nodup_of_length_eq_of_all_mem [DecidableEq α] (as bs : List α) (nodup : as.Nodup) (eq_length : as.length = bs.length) (all_mem : ∀ e, e ∈ as -> e ∈ bs) : ∀ e, e ∈ as ↔ e ∈ bs := by
-    intro e
-    constructor
-    . apply all_mem
-    . intro mem_bs
-      induction as generalizing bs e with
-      | nil => cases bs; simp at mem_bs; simp at eq_length
-      | cons a as ih =>
-        let bs_without_a := bs.erase a
-        simp at nodup
-        specialize ih
-          bs_without_a
-          nodup.right
-          (by rw [List.length_erase_of_mem, ← eq_length]; simp; apply all_mem; simp)
-          (by intro c c_mem; rw [List.mem_erase_of_ne]; apply all_mem; simp [c_mem]; intro contra; rw [contra] at c_mem; apply nodup.left; exact c_mem)
-        cases Decidable.em (e = a) with
-        | inl eq => simp [eq]
-        | inr neq =>
-          simp; apply Or.inr
-          apply ih
-          rw [List.mem_erase_of_ne]
-          exact mem_bs
-          exact neq
 end List
 
 namespace Function
 
-  def image_set (f : α -> β) (A : Set α) : Set β := fun b => ∃ a, a ∈ A ∧ f a = b
+/-!
+### Injectivity and Surjectivity
 
-  def injective_for_domain_set (f : α -> β) (domain : Set α) : Prop := ∀ a a', a ∈ domain -> a' ∈ domain -> f a = f a' -> a = a'
-  def surjective_for_domain_and_image_set (f : α -> β) (domain : Set α) (image : Set β) : Prop := ∀ b, b ∈ image -> ∃ a, a ∈ domain ∧ f a = b
+We define what it means for a function to be injective or surjective restricted to a given domain and image, given as either a list or set.
+Intuitively, results involving the list versions most likely have an implicit requirement for domain and image being finite whereas results stated for the set version do not have this requirement.
 
-  theorem injective_of_injective_compose (f : α -> β) (g : β -> γ) (domain : Set α) :
-      injective_for_domain_set (g ∘ f) domain -> injective_for_domain_set f domain := by
-    intro inj a a' a_dom a'_dom image_eq
-    apply inj a a' a_dom a'_dom
-    simp [image_eq]
+We found our more suitable than using `Function.Injective` and `Function.Sufjective` because this would require us to consider appropriate subtypes and also since there barely seem to be theorems in the standard library (outside Mathlib).
+We might rework those definitions in the future though. I think a couple of (small) things can be cleaned up here but this is not the highest priprity.
+Maybe this should even move to the BasicLeanDatastructures repo since there are really just general results over functions.
+-/
 
-  theorem surjective_of_surjective_from_subset (f : α -> β) (domain : Set α) (image : Set β) :
-      f.surjective_for_domain_and_image_set domain image ->
-      ∀ domain', domain ⊆ domain' -> f.surjective_for_domain_and_image_set domain' image := by
-    intro surj dom' dom'_sub b b_mem
-    rcases surj b b_mem with ⟨a, a_mem, a_eq⟩
+/-- The image of a function for a given domain set. -/
+def image_set (f : α -> β) (A : Set α) : Set β := A.map f
+
+/-- A function is injective on a given domain set if for each two elements of the given domain, the mapping of both elements being the same implies the elements being the same. -/
+def injective_for_domain_set (f : α -> β) (domain : Set α) : Prop := ∀ a a', a ∈ domain -> a' ∈ domain -> f a = f a' -> a = a'
+
+/-- A function is surjective on a given domain set and image set if for each element of the image, there exists an element in the domain that maps to the desired image element. -/
+def surjective_for_domain_and_image_set (f : α -> β) (domain : Set α) (image : Set β) : Prop := ∀ b, b ∈ image -> ∃ a, a ∈ domain ∧ f a = b
+
+/-- The image of a function for a given domain list. -/
+def image [DecidableEq β] (f : α -> β) (l : List α) : List β := (l.map f).eraseDupsKeepRight
+
+/-- A function is injective on a given domain list if for each two elements of the given domain, the mapping of both elements being the same implies the elements being the same. -/
+def injective_for_domain_list (f : α -> β) (domain : List α) : Prop := ∀ a a', a ∈ domain -> a' ∈ domain -> f a = f a' -> a = a'
+
+/-- A function is surjective on a given domain list and image list if for each element of the image, there exists an element in the domain that maps to the desired image element. -/
+def surjective_for_domain_and_image_list (f : α -> β) (domain : List α) (image : List β) : Prop := ∀ b, b ∈ image -> ∃ a, a ∈ domain ∧ f a = b
+
+/-- If the composition of two mappings is injective, then the first one must be injective. -/
+theorem injective_of_injective_compose (f : α -> β) (g : β -> γ) (domain : Set α) :
+    injective_for_domain_set (g ∘ f) domain -> injective_for_domain_set f domain := by
+  intro inj a a' a_dom a'_dom image_eq
+  apply inj a a' a_dom a'_dom
+  simp [image_eq]
+
+/-- If a mapping is surjective for a domain and image, then the same holds for any superset of the domain. -/
+theorem surjective_of_surjective_from_subset (f : α -> β) (domain : Set α) (image : Set β) :
+    f.surjective_for_domain_and_image_set domain image ->
+    ∀ domain', domain ⊆ domain' -> f.surjective_for_domain_and_image_set domain' image := by
+  intro surj dom' dom'_sub b b_mem
+  rcases surj b b_mem with ⟨a, a_mem, a_eq⟩
+  exists a
+  constructor
+  . apply dom'_sub; exact a_mem
+  . exact a_eq
+
+/-- If the composition of two mappings is surjective for a domain and image, then the second one must be surjective on the same image and the domain that is the image of the first function. -/
+theorem surjective_of_surjective_compose (f : α -> β) (g : β -> γ) (domain : Set α) (image : Set γ) :
+    surjective_for_domain_and_image_set (g ∘ f) domain image ->
+    surjective_for_domain_and_image_set g (f.image_set domain) image := by
+  intro surj b b_mem
+  rcases surj b b_mem with ⟨a, a_mem, a_eq⟩
+  exists f a
+  constructor
+  . exists a
+  . exact a_eq
+
+/-- The injectivity definitions for set and list are interchangeable. -/
+theorem injective_set_list_equiv (f : α -> β) (domain_set : Set α) (domain_list : List α) (eq : ∀ e, e ∈ domain_list ↔ e ∈ domain_set) : f.injective_for_domain_set domain_set ↔ f.injective_for_domain_list domain_list := by
+  constructor
+  . intro h a a' a_mem a'_mem f_eq
+    apply h
+    . rw [← eq]; assumption
+    . rw [← eq]; assumption
+    . exact f_eq
+  . intro h a a' a_mem a'_mem f_eq
+    apply h
+    . rw [eq]; assumption
+    . rw [eq]; assumption
+    . exact f_eq
+
+/-- The surjectivity definitions for set and list are interchangeable. -/
+theorem surjective_set_list_equiv (f : α -> β)
+    (domain_set : Set α) (domain_list : List α) (eq_domain : ∀ e, e ∈ domain_list ↔ e ∈ domain_set)
+    (image_set : Set β) (image_list : List β) (eq_image : ∀ e, e ∈ image_list ↔ e ∈ image_set) :
+    f.surjective_for_domain_and_image_set domain_set image_set ↔ f.surjective_for_domain_and_image_list domain_list image_list := by
+  constructor
+  . intro h b b_mem
+    specialize h b (by rw [← eq_image]; exact b_mem)
+    rcases h with ⟨a, a_mem, a_eq⟩
     exists a
     constructor
-    . apply dom'_sub; exact a_mem
+    . rw [eq_domain]; exact a_mem
+    . exact a_eq
+  . intro h b b_mem
+    specialize h b (by rw [eq_image]; exact b_mem)
+    rcases h with ⟨a, a_mem, a_eq⟩
+    exists a
+    constructor
+    . rw [← eq_domain]; exact a_mem
     . exact a_eq
 
-  theorem surjective_of_surjective_compose (f : α -> β) (g : β -> γ) (domain : Set α) (image : Set γ) :
-      surjective_for_domain_and_image_set (g ∘ f) domain image ->
-      surjective_for_domain_and_image_set g (f.image_set domain) image := by
-    intro surj b b_mem
-    rcases surj b b_mem with ⟨a, a_mem, a_eq⟩
-    exists f a
-    constructor
-    . exists a
-    . exact a_eq
+/-- If a mapping is injective on a domain of the form `hd::tl`, then it is injective on `tl`. -/
+theorem injective_for_domain_list_cons (f : α -> β) (hd : α) (tl : List α) : f.injective_for_domain_list (hd::tl) -> f.injective_for_domain_list tl := by
+  intro h a a' a_mem a'_mem eq
+  apply h
+  . simp [a_mem]
+  . simp [a'_mem]
+  . exact eq
 
-  def injective_for_domain_list (f : α -> β) (domain : List α) : Prop := ∀ a a', a ∈ domain -> a' ∈ domain -> f a = f a' -> a = a'
-  def surjective_for_domain_and_image_list (f : α -> β) (domain : List α) (image : List β) : Prop := ∀ b, b ∈ image -> ∃ a, a ∈ domain ∧ f a = b
+/-- The mapping of each domain element occurs in the `image`. -/
+theorem mapping_mem_image_of_mem [DecidableEq β] (f : α -> β) (domain : List α) : ∀ a, a ∈ domain -> f a ∈ (image f domain) := by
+  intro a a_mem; apply (List.mem_eraseDupsKeepRight _ _).mpr; apply List.mem_map_of_mem; exact a_mem
 
-  theorem injective_set_list_equiv (f : α -> β) (domain_set : Set α) (domain_list : List α) (eq : ∀ e, e ∈ domain_list ↔ e ∈ domain_set) : f.injective_for_domain_set domain_set ↔ f.injective_for_domain_list domain_list := by
-    constructor
-    . intro h a a' a_mem a'_mem f_eq
-      apply h
-      . rw [← eq]; assumption
-      . rw [← eq]; assumption
-      . exact f_eq
-    . intro h a a' a_mem a'_mem f_eq
-      apply h
-      . rw [eq]; assumption
-      . rw [eq]; assumption
-      . exact f_eq
+/-- The `image` has no duplicates. -/
+theorem nodup_image [DecidableEq β] (f : α -> β) (domain : List α) : (image f domain).Nodup := by apply List.nodup_eraseDupsKeepRight
 
-  theorem surjective_set_list_equiv (f : α -> β)
-      (domain_set : Set α) (domain_list : List α) (eq_domain : ∀ e, e ∈ domain_list ↔ e ∈ domain_set)
-      (image_set : Set β) (image_list : List β) (eq_image : ∀ e, e ∈ image_list ↔ e ∈ image_set) :
-      f.surjective_for_domain_and_image_set domain_set image_set ↔ f.surjective_for_domain_and_image_list domain_list image_list := by
-    constructor
-    . intro h b b_mem
-      specialize h b (by rw [← eq_image]; exact b_mem)
-      rcases h with ⟨a, a_mem, a_eq⟩
-      exists a
-      constructor
-      . rw [eq_domain]; exact a_mem
-      . exact a_eq
-    . intro h b b_mem
-      specialize h b (by rw [eq_image]; exact b_mem)
-      rcases h with ⟨a, a_mem, a_eq⟩
-      exists a
-      constructor
-      . rw [← eq_domain]; exact a_mem
-      . exact a_eq
+/-- The `image` has at most as many elements as the domain. -/
+theorem length_image [DecidableEq β] (f : α -> β) (domain : List α) : (image f domain).length ≤ domain.length := by
+  have : domain.length = (domain.map f).length := by rw [List.length_map]
+  rw [this]
+  apply List.length_le_of_nodup_of_all_mem
+  . apply nodup_image
+  . simp [image, List.mem_eraseDupsKeepRight]
 
-  theorem injective_for_domain_list_cons (f : α -> β) (hd : α) (tl : List α) : f.injective_for_domain_list (hd::tl) -> f.injective_for_domain_list tl := by
-    intro h a a' a_mem a'_mem eq
-    apply h
-    . simp [a_mem]
-    . simp [a'_mem]
-    . exact eq
+/-- Every mapping is always surjective on its own `image`. -/
+theorem surjective_on_own_image [DecidableEq β] (f : α -> β) (domain : List α) : f.surjective_for_domain_and_image_list domain (image f domain) := by
+  intro b b_mem; simp only [image, List.mem_eraseDupsKeepRight, List.mem_map] at b_mem; exact b_mem
 
-  def image [DecidableEq β] (f : α -> β) : List α -> List β
-  | [] => []
-  | hd::tl =>
-    let tl_img := image f tl
-    if f hd ∈ tl_img then tl_img else (f hd)::tl_img
+/-- If a mapping is closed, then its image is fully contained in its domain. -/
+theorem image_contained_of_closed [DecidableEq α] (f : α -> α) (domain : List α) (closed : ∀ e, e ∈ domain -> f e ∈ domain) : ∀ e, e ∈ image f domain -> e ∈ domain := by
+  intro b b_mem
+  rcases surjective_on_own_image f domain b b_mem with ⟨a, a_mem, a_eq⟩
+  rw [← a_eq]
+  apply closed
+  exact a_mem
 
-  theorem mapping_mem_image_of_mem [DecidableEq β] (f : α -> β) (domain : List α) : ∀ a, a ∈ domain -> f a ∈ (image f domain) := by
-    intro a a_mem
+/-- Given a mapping and a domain list without duplicates, the mapping in injective on the domain if and only if the `image` contains the same number of elements as the domain.  -/
+theorem injective_iff_length_image_eq_of_nodup [DecidableEq β] (f : α -> β) (domain : List α) (nodup : domain.Nodup) : f.injective_for_domain_list domain ↔ (image f domain).length = domain.length := by
+  -- TODO: we can probably shorten this proof a lot by proving appropriate results about List.eraseDupsKeepRight
+  constructor
+  . intro inj
     induction domain with
-    | nil => simp at a_mem
-    | cons hd tl ih =>
-      simp [image]
-      cases Decidable.em (f hd ∈ image f tl) with
-      | inl hd_mem => simp [hd_mem]; cases a_mem; exact hd_mem; apply ih; assumption
-      | inr hd_not_mem => simp [hd_not_mem]; cases a_mem; apply Or.inl; rfl; apply Or.inr; apply ih; assumption
-
-  theorem nodup_image [DecidableEq β] (f : α -> β) (domain : List α) : (image f domain).Nodup := by
-    induction domain with
-    | nil => simp [image]
+    | nil => simp [image, List.eraseDupsKeepRight]
     | cons hd tl ih =>
       cases Decidable.em (f hd ∈ image f tl) with
-      | inl hd_mem => simp [image, hd_mem]; exact ih
-      | inr hd_not_mem => simp [image, hd_not_mem]; exact ih
-
-  theorem length_image [DecidableEq β] (f : α -> β) (domain : List α) : (image f domain).length ≤ domain.length := by
-    induction domain with
-    | nil => simp [image]
-    | cons hd tl ih => simp [image]; split; apply Nat.le_trans; exact ih; simp; simp; exact ih
-
-  theorem surjective_on_own_image [DecidableEq β] (f : α -> β) (domain : List α) : f.surjective_for_domain_and_image_list domain (image f domain) := by
-    induction domain with
-    | nil => simp [surjective_for_domain_and_image_list, image]
-    | cons hd tl ih =>
-      intro b b_mem
-      cases Decidable.em (f hd ∈ image f tl) with
-      | inl hd_mem => simp [image, hd_mem] at b_mem; rcases ih b b_mem with ⟨a, ha⟩; exists a; simp [ha]
+      | inl hd_mem =>
+        apply False.elim
+        simp only [List.nodup_cons] at nodup
+        apply nodup.left
+        rcases surjective_on_own_image f tl (f hd) hd_mem with ⟨a, a_mem, a_eq⟩
+        specialize inj a hd (by simp [a_mem]) (by simp) a_eq
+        rw [← inj]
+        exact a_mem
       | inr hd_not_mem =>
-        simp [image, hd_not_mem] at b_mem
-        cases b_mem with
-        | inr b_mem => rcases ih b b_mem with ⟨a, ha⟩; exists a; simp [ha]
-        | inl b_mem => exists hd; simp [b_mem]
+        simp only [image, List.mem_eraseDupsKeepRight] at hd_not_mem
+        simp only [image, List.map_cons, List.eraseDupsKeepRight, hd_not_mem, ↓reduceIte, List.length_cons, Nat.add_right_cancel_iff]
+        apply ih
+        . simp only [List.nodup_cons] at nodup; exact nodup.right
+        . apply injective_for_domain_list_cons; exact inj
+  . intro length_eq
+    induction domain with
+    | nil => simp [injective_for_domain_list]
+    | cons hd tl ih =>
+      cases Decidable.em (f hd ∈ image f tl) with
+      | inl hd_mem =>
+        simp only [image, List.mem_eraseDupsKeepRight] at hd_mem
+        simp only [image, List.map_cons, List.eraseDupsKeepRight, hd_mem, ↓reduceIte, List.length_cons] at length_eq
+        have contra := length_image f tl
+        simp only [image, length_eq] at contra
+        simp [Nat.succ_le_iff] at contra
+      | inr hd_not_mem =>
+        simp only [image, List.mem_eraseDupsKeepRight] at hd_not_mem
+        simp only [image, List.map_cons, List.eraseDupsKeepRight, hd_not_mem, ↓reduceIte, List.length_cons, Nat.add_right_cancel_iff] at length_eq
+        intro a a' a_mem a'_mem eq
+        rw [List.mem_cons] at a_mem
+        rw [List.mem_cons] at a'_mem
+        cases a_mem with
+        | inl a_mem => cases a'_mem with
+          | inl a'_mem => rw [a_mem, a'_mem]
+          | inr a'_mem =>
+            apply False.elim
+            apply hd_not_mem
+            rw [← a_mem, eq]
+            apply List.mem_map_of_mem
+            exact a'_mem
+        | inr a_mem => cases a'_mem with
+          | inl a'_mem =>
+            apply False.elim
+            apply hd_not_mem
+            rw [← a'_mem, ← eq]
+            apply List.mem_map_of_mem
+            exact a_mem
+          | inr a'_mem =>
+            simp only [List.nodup_cons] at nodup
+            specialize ih nodup.right length_eq
+            apply ih <;> assumption
 
-  theorem image_contained_of_closed [DecidableEq α] (f : α -> α) (domain : List α) (closed : ∀ e, e ∈ domain -> f e ∈ domain) : ∀ e, e ∈ image f domain -> e ∈ domain := by
-    intro b b_mem
-    rcases surjective_on_own_image f domain b b_mem with ⟨a, a_mem, a_eq⟩
+/-- A mapping is surjective on a given domain and image if and only if the given image is contained in the actual image of the mapping. -/
+theorem surjective_on_target_iff_all_in_image [DecidableEq β] (f : α -> β) (domain : List α) (target_image : List β) : f.surjective_for_domain_and_image_list domain target_image ↔ ∀ b, b ∈ target_image -> b ∈ image f domain := by
+  constructor
+  . intro surj b b_mem
+    specialize surj b b_mem
+    rcases surj with ⟨a, a_mem, a_eq⟩
     rw [← a_eq]
-    apply closed
+    apply mapping_mem_image_of_mem
     exact a_mem
+  . intro h b b_mem
+    apply surjective_on_own_image
+    apply h
+    exact b_mem
 
-  theorem injective_iff_length_image_eq_of_nodup [DecidableEq β] (f : α -> β) (domain : List α) (nodup : domain.Nodup) : f.injective_for_domain_list domain ↔ (image f domain).length = domain.length := by
-    constructor
-    . intro inj
-      induction domain with
-      | nil => simp [image]
-      | cons hd tl ih =>
-        cases Decidable.em (f hd ∈ image f tl) with
-        | inl hd_mem =>
-          apply False.elim
-          simp at nodup
-          apply nodup.left
-          rcases surjective_on_own_image f tl (f hd) hd_mem with ⟨a, a_mem, a_eq⟩
-          specialize inj a hd (by simp [a_mem]) (by simp) a_eq
-          rw [← inj]
-          exact a_mem
-        | inr hd_not_mem =>
-          simp [image, hd_not_mem]
-          apply ih
-          . simp at nodup; exact nodup.right
-          . apply injective_for_domain_list_cons; exact inj
-    . intro length_eq
-      induction domain with
-      | nil => simp [injective_for_domain_list]
-      | cons hd tl ih =>
-        cases Decidable.em (f hd ∈ image f tl) with
-        | inl hd_mem =>
-          simp [image, hd_mem] at length_eq
-          have contra := length_image f tl
-          rw [length_eq] at contra
-          simp [Nat.succ_le_iff] at contra
-        | inr hd_not_mem =>
-          simp [image, hd_not_mem] at length_eq
-          intro a a' a_mem a'_mem eq
-          cases a_mem
-          . cases a'_mem
-            . rfl
-            . apply False.elim
-              apply hd_not_mem
-              rw [eq]
-              apply mapping_mem_image_of_mem
-              assumption
-          . cases a'_mem
-            . apply False.elim
-              apply hd_not_mem
-              rw [← eq]
-              apply mapping_mem_image_of_mem
-              assumption
-            . simp at nodup
-              specialize ih nodup.right length_eq
-              apply ih <;> assumption
+/-- Given a single list without duplicates that represents both domain and image, if a mapping is surjective, then it is injective. -/
+theorem injective_of_surjective_of_nodup [DecidableEq α] (f : α -> α) (l : List α) (nodup : l.Nodup) : f.surjective_for_domain_and_image_list l l -> f.injective_for_domain_list l := by
+  intro surj
+  rw [surjective_on_target_iff_all_in_image] at surj
+  rw [injective_iff_length_image_eq_of_nodup _ _ nodup]
+  rw [Nat.eq_iff_le_and_ge]
+  constructor
+  . exact length_image f l
+  . exact List.length_le_of_nodup_of_all_mem l (image f l) nodup surj
 
-  theorem surjective_on_target_iff_all_in_image [DecidableEq β] (f : α -> β) (domain : List α) (target_image : List β) : f.surjective_for_domain_and_image_list domain target_image ↔ ∀ b, b ∈ target_image -> b ∈ image f domain := by
-    constructor
-    . intro surj b b_mem
-      specialize surj b b_mem
-      rcases surj with ⟨a, a_mem, a_eq⟩
-      rw [← a_eq]
-      apply mapping_mem_image_of_mem
-      exact a_mem
-    . intro h b b_mem
-      apply surjective_on_own_image
-      apply h
-      exact b_mem
+/-- Given a single list without duplicates that represents both domain and image, if a mapping closed on the list, then the mapping is injective if and only if it is surjective. -/
+theorem injective_iff_surjective_of_nodup_of_closed [DecidableEq α] (f : α -> α) (l : List α) (nodup : l.Nodup) (closed : ∀ e, e ∈ l -> f e ∈ l) : f.injective_for_domain_list l ↔ f.surjective_for_domain_and_image_list l l := by
+  constructor
+  . intro inj
 
-  theorem injective_of_surjective_of_nodup [DecidableEq α] (f : α -> α) (l : List α) (nodup : l.Nodup) : f.surjective_for_domain_and_image_list l l -> f.injective_for_domain_list l := by
-    intro surj
-    rw [surjective_on_target_iff_all_in_image] at surj
-    rw [injective_iff_length_image_eq_of_nodup _ _ nodup]
-    rw [Nat.eq_iff_le_and_ge]
-    constructor
-    . exact length_image f l
-    . exact List.length_le_of_nodup_of_all_mem l (image f l) nodup surj
+    have : ∀ e, e ∈ image f l ↔ e ∈ l := by
+      apply List.equiv_of_nodup_of_length_eq_of_all_mem
+      . apply nodup_image
+      . rw [injective_iff_length_image_eq_of_nodup] at inj
+        rw [inj]
+        exact nodup
+      . intro e e_mem
+        apply image_contained_of_closed
+        . exact closed
+        . exact e_mem
 
-  theorem injective_iff_surjective_of_nodup_of_closed [DecidableEq α] (f : α -> α) (l : List α) (nodup : l.Nodup) (closed : ∀ e, e ∈ l -> f e ∈ l) : f.injective_for_domain_list l ↔ f.surjective_for_domain_and_image_list l l := by
-    constructor
-    . intro inj
+    rw [surjective_on_target_iff_all_in_image]
+    intro b
+    apply (this b).mpr
+  . apply injective_of_surjective_of_nodup; exact nodup
 
-      have : ∀ e, e ∈ image f l ↔ e ∈ l := by
-        apply List.equiv_of_nodup_of_length_eq_of_all_mem
-        . apply nodup_image
-        . rw [injective_iff_length_image_eq_of_nodup] at inj
-          rw [inj]
-          exact nodup
-        . intro e e_mem
-          apply image_contained_of_closed
-          . exact closed
-          . exact e_mem
-
-      rw [surjective_on_target_iff_all_in_image]
-      intro b
-      apply (this b).mpr
-    . apply injective_of_surjective_of_nodup; exact nodup
-
-  theorem closed_of_injective_of_surjective_of_nodup [DecidableEq α] (f : α -> α) (l : List α) (nodup : l.Nodup) : f.injective_for_domain_list l -> f.surjective_for_domain_and_image_list l l -> ∀ e, e ∈ l -> f e ∈ l := by
-    intro inj surj
-    intro e e_mem
-    rw [List.equiv_of_nodup_of_length_eq_of_all_mem l (image f l) nodup]
-    . apply mapping_mem_image_of_mem; exact e_mem
-    . rw [(injective_iff_length_image_eq_of_nodup f l nodup).mp inj]
-    . exact (surjective_on_target_iff_all_in_image f l l).mp surj
+/-- Given a single list without duplicates that represents both domain and image, if a mapping both injective and surjective, then is must be closed on the list. -/
+theorem closed_of_injective_of_surjective_of_nodup [DecidableEq α] (f : α -> α) (l : List α) (nodup : l.Nodup) : f.injective_for_domain_list l -> f.surjective_for_domain_and_image_list l l -> ∀ e, e ∈ l -> f e ∈ l := by
+  intro inj surj
+  intro e e_mem
+  rw [List.equiv_of_nodup_of_length_eq_of_all_mem l (image f l) nodup]
+  . apply mapping_mem_image_of_mem; exact e_mem
+  . rw [(injective_iff_length_image_eq_of_nodup f l nodup).mp inj]
+  . exact (surjective_on_target_iff_all_in_image f l l).mp surj
 
 end Function
 
 namespace GroundTermMapping
 
-  variable {sig : Signature} [DecidableEq sig.C] [DecidableEq sig.V] [DecidableEq sig.P]
+/-!
+## Strong GroundTermMappings (and Homomorphisms)
 
-  def strong (h : GroundTermMapping sig) (domain : Set (GroundTerm sig)) (A B : FactSet sig) : Prop :=
-    ∀ (e : Fact sig), (∀ t, t ∈ e.terms -> t ∈ domain) -> ¬ e ∈ A -> ¬ (h.applyFact e) ∈ B
+Intuitively, a homomorphism is `strong` if it not only retains membership but also non-membership.
+We define being `strong` as a standalone property for `GroundTermMapping`s
+without requiring any additional properties for the underlying `GroundTermMapping`.
+-/
 
-  theorem strong_of_compose_strong (g h : GroundTermMapping sig) (domain : Set (GroundTerm sig)) (A B C : FactSet sig) :
-      h.isHomomorphism B C -> GroundTermMapping.strong (h ∘ g) domain A C -> g.strong domain A B := by
-    intro h_hom compose_strong
-    intro e e_dom e_not_mem_a e_mem_b
-    apply compose_strong e
-    . exact e_dom
-    . exact e_not_mem_a
-    . apply h_hom.right (GroundTermMapping.applyFact (h ∘ g) e)
-      exists (g.applyFact e)
-      constructor
-      . exact e_mem_b
-      . unfold applyFact
-        rw [TermMapping.apply_generalized_atom_compose]
-        simp
+variable {sig : Signature} [DecidableEq sig.C] [DecidableEq sig.V] [DecidableEq sig.P]
+
+/-- A `GroundTermMapping` is strong for `FactSet`s A and B if each element not in A, its mapping is not in B. However, we only demand this for elements that only feature terms from a given domain because we do not want to care about the mapping of terms outside the domain. -/
+def strong (h : GroundTermMapping sig) (domain : Set (GroundTerm sig)) (A B : FactSet sig) : Prop :=
+  ∀ (e : Fact sig), (∀ t, t ∈ e.terms -> t ∈ domain) -> ¬ e ∈ A -> ¬ (h.applyFact e) ∈ B
+
+/-- If the composition of two mappings is strong from A to C and the second mapping is a homomorphism from B to C, then the first mapping is strong from A to B. -/
+theorem strong_of_compose_strong (g h : GroundTermMapping sig) (domain : Set (GroundTerm sig)) (A B C : FactSet sig) :
+    h.isHomomorphism B C -> GroundTermMapping.strong (h ∘ g) domain A C -> g.strong domain A B := by
+  intro h_hom compose_strong
+  intro e e_dom e_not_mem_a e_mem_b
+  apply compose_strong e
+  . exact e_dom
+  . exact e_not_mem_a
+  . apply h_hom.right (GroundTermMapping.applyFact (h ∘ g) e)
+    exists (g.applyFact e)
+    constructor
+    . exact e_mem_b
+    . unfold applyFact
+      rw [TermMapping.apply_generalized_atom_compose]
+      simp
 
 end GroundTermMapping
-
-
-section HomomorphismRepetition
-
--- TODO: I think a lot of this can be generalized to arbitrary Functions
 
 namespace GroundTermMapping
 
-  variable {sig : Signature} [DecidableEq sig.C] [DecidableEq sig.V]
+-- TODO: I think a lot of the following can be generalized to arbitrary Functions
 
-  def repeat_hom (h : GroundTermMapping sig) : Nat -> GroundTermMapping sig
-  | .zero => id
-  | .succ j => h ∘ (h.repeat_hom j)
+/-!
+## Repetition of GroundTermMappings (and Homomorphisms)
 
-  theorem repeat_hom_swap (h : GroundTermMapping sig) (i : Nat) : ∀ t, h (h.repeat_hom i t) = (h.repeat_hom i) (h t) := by
-    intro t
-    induction i with
-    | zero => unfold repeat_hom; simp
-    | succ i ih =>
-      unfold repeat_hom
-      simp
-      rw [ih]
+In general, we can define what it means to apply a function a given number of times.
+This is particularly useful for `GroundTermMapping`s that are endomorphisms, i.e. homomorphisms from one structure into the same structure.
+We can show some nice properties for such repetitions. For example, a repeated endomorphisms is still an endomorphisms.
+-/
 
-  theorem repeat_hom_add (h : GroundTermMapping sig) (n m : Nat) : ∀ t, h.repeat_hom (n + m) t = h.repeat_hom n (h.repeat_hom m t) := by
-    intro t
-    induction m with
-    | zero => simp [repeat_hom]
-    | succ m ih =>
-      conv => left; unfold repeat_hom
-      conv => right; right; unfold repeat_hom
-      simp
-      rw [ih]
-      rw [h.repeat_hom_swap]
+variable {sig : Signature} [DecidableEq sig.C] [DecidableEq sig.V]
 
-  theorem repeat_hom_cycle_mul (h : GroundTermMapping sig) (t : GroundTerm sig) (n : Nat) : h.repeat_hom n t = t -> ∀ m, h.repeat_hom (n * m) t = t := by
-    intro cycle m
-    induction m with
-    | zero => simp [repeat_hom]
-    | succ m ih =>
-      rw [Nat.mul_add]
-      rw [repeat_hom_add]
-      simp
-      rw [cycle, ih]
+/-- Repetition of a `GroundTermMapping` defined in the obvious way. Repeating zero times is defined as the id function. -/
+def repeat_hom (h : GroundTermMapping sig) : Nat -> GroundTermMapping sig
+| .zero => id
+| .succ j => h ∘ (h.repeat_hom j)
 
-  theorem repeat_hom_move_cycle (h : GroundTermMapping sig) (t : GroundTerm sig) (n : Nat) : h.repeat_hom n t = t -> ∀ s m, h.repeat_hom m t = s -> h.repeat_hom n s = s := by
-    intro cycle s m reaches_s
-    induction m generalizing t with
-    | zero => simp [repeat_hom] at reaches_s; rw [← reaches_s]; exact cycle
-    | succ m ih =>
-      apply ih (h t)
-      . rw [← h.repeat_hom_swap]
-        rw [cycle]
-      . simp [repeat_hom] at reaches_s
-        rw [h.repeat_hom_swap] at reaches_s
-        exact reaches_s
+/-- It does not mapper if we apply add one more repetition on the left or the right. -/
+theorem repeat_hom_swap (h : GroundTermMapping sig) (i : Nat) : ∀ t, h (h.repeat_hom i t) = (h.repeat_hom i) (h t) := by
+  intro t
+  induction i with
+  | zero => unfold repeat_hom; simp
+  | succ i ih => unfold repeat_hom; simp [ih]
 
-  theorem repeat_each_reaches_self_of_each_reachable (h : GroundTermMapping sig) (ts : List (GroundTerm sig)) (each_reachable : ∀ t, t ∈ ts -> ∃ k, 1 ≤ k ∧ ∃ s, s ∈ ts ∧ (h.repeat_hom k) s = t) : (∀ s, s ∈ ts -> ∃ l, 1 ≤ l ∧ (h.repeat_hom l) s = s) := by
-    induction ts with
-    | nil => simp
-    | cons hd tl ih =>
-      specialize ih (by
-        intro t t_mem
-        have each_reachable_for_t := each_reachable t (by simp [t_mem])
-        rcases each_reachable_for_t with ⟨k, k_le, s, s_mem, s_eq⟩
-        simp at s_mem
-        cases s_mem with
-        | inr s_mem => exists k; constructor; exact k_le; exists s
-        | inl s_mem =>
-          have each_reachable_for_s := each_reachable s (by simp [s_mem])
-          rcases each_reachable_for_s with ⟨l, l_le, u, u_mem, u_eq⟩
-          simp at u_mem
-          cases u_mem with
-          | inl u_mem =>
-            exists (((k / l) + 1) * l)
-            constructor
-            .
-              rw [Nat.add_mul]
-              apply Nat.le_trans
-              . exact k_le
-              . apply Nat.le_of_lt
-                simp
-                -- NOTE: taken from https://github.com/leanprover-community/mathlib4/blob/3f813de52d8cffaa73e27edd62364eec90eac633/Mathlib/Data/Nat/Defs.lean#L473-L474
-                rw [← Nat.succ_mul, ← Nat.div_lt_iff_lt_mul (by apply Nat.lt_of_succ_le; exact l_le)]; exact Nat.lt_succ_self _
-            . exists t
-              constructor
-              . exact t_mem
-              . apply h.repeat_hom_move_cycle s
-                . rw [Nat.mul_comm]
-                  apply h.repeat_hom_cycle_mul
-                  rw [u_mem, ← s_mem] at u_eq
-                  exact u_eq
-                . exact s_eq
-          | inr u_mem =>
-            exists (k + l)
-            constructor
-            . apply Nat.le_add_right_of_le; exact k_le
-            . exists u
-              constructor
-              . exact u_mem
-              . rw [GroundTermMapping.repeat_hom_add]
-                rw [u_eq, s_eq]
-      )
+/-- A (n+m)-times repetition can be split into the composition of an m-times repetition followed by an n-times repetition. -/
+theorem repeat_hom_add (h : GroundTermMapping sig) (n m : Nat) : ∀ t, h.repeat_hom (n + m) t = h.repeat_hom n (h.repeat_hom m t) := by
+  intro t
+  induction m with
+  | zero => simp [repeat_hom]
+  | succ m ih =>
+    conv => left; unfold repeat_hom
+    conv => right; right; unfold repeat_hom
+    simp [ih, h.repeat_hom_swap]
 
-      intro s s_mem
-      simp at s_mem
-      cases s_mem with
-      | inl s_mem =>
-        specialize each_reachable s (by rw [s_mem]; simp)
-        rcases each_reachable with ⟨k, k_le, t, t_mem, t_eq⟩
-        simp at t_mem
-        cases t_mem with
-        | inl t_mem => exists k; constructor; exact k_le; rw [t_mem, ← s_mem] at t_eq; exact t_eq
-        | inr t_mem =>
-          specialize ih t t_mem
-          rcases ih with ⟨l, l_le, ih⟩
-          exists l
-          constructor
-          . exact l_le
-          . apply h.repeat_hom_move_cycle t
-            . exact ih
-            . exact t_eq
-      | inr s_mem =>
-        apply ih
-        exact s_mem
+/-- If some repetition maps a term to itself, then each multiple of the repetition count must also map the term to itself. -/
+theorem repeat_hom_cycle_mul (h : GroundTermMapping sig) (t : GroundTerm sig) (n : Nat) : h.repeat_hom n t = t -> ∀ m, h.repeat_hom (n * m) t = t := by
+  intro cycle m
+  induction m with
+  | zero => simp [repeat_hom]
+  | succ m ih =>
+    rw [Nat.mul_add]
+    rw [repeat_hom_add]
+    simp [cycle, ih]
 
-  theorem repeat_globally_of_each_repeats (h : GroundTermMapping sig) (ts : List (GroundTerm sig)) (each_repeats : ∀ s, s ∈ ts -> ∃ l, 1 ≤ l ∧ (h.repeat_hom l) s = s) :
-      ∃ l, 1 ≤ l ∧ ∀ s, s ∈ ts -> (h.repeat_hom l) s = s := by
-    induction ts with
-    | nil => exists 1; simp
-    | cons hd tl ih =>
-      specialize ih (by intro s s_mem; apply each_repeats; simp [s_mem])
-      rcases ih with ⟨l_ih, l_ih_le, ih⟩
-      rcases each_repeats hd (by simp) with ⟨l_hd, l_hd_le, each_repeats⟩
-      exists l_hd * l_ih
-      constructor
-      . apply Nat.le_trans; exact l_hd_le; apply Nat.le_mul_of_pos_right; apply Nat.lt_of_succ_le; exact l_ih_le
-      . intro s s_mem
-        simp at s_mem
-        cases s_mem with
-        | inl s_mem => rw [s_mem, h.repeat_hom_cycle_mul]; exact each_repeats
-        | inr s_mem => specialize ih s s_mem; rw [Nat.mul_comm, h.repeat_hom_cycle_mul]; exact ih
+/-- If some repetition maps a term to itself, then for each other term that is part of the loop, the same number of repetitions also maps that one to itself. -/
+theorem repeat_hom_move_cycle (h : GroundTermMapping sig) (t : GroundTerm sig) (n : Nat) : h.repeat_hom n t = t -> ∀ s m, h.repeat_hom m t = s -> h.repeat_hom n s = s := by
+  intro cycle s m reaches_s
+  induction m generalizing t with
+  | zero => simp only [repeat_hom, id_eq] at reaches_s; rw [← reaches_s]; exact cycle
+  | succ m ih =>
+    apply ih (h t)
+    . rw [← h.repeat_hom_swap]
+      rw [cycle]
+    . simp only [repeat_hom, Function.comp_apply] at reaches_s
+      rw [h.repeat_hom_swap] at reaches_s
+      exact reaches_s
 
-  theorem exists_repetition_that_is_inverse_of_surj (h : GroundTermMapping sig) (ts : List (GroundTerm sig)) (surj : h.surjective_for_domain_and_image_list ts ts) : ∃ k, ∀ t, t ∈ ts -> (h.repeat_hom k) (h t) = t := by
-    have each_repeats := h.repeat_each_reaches_self_of_each_reachable ts (by
+/-- Consider a list of terms. If each term is reachable by some number of repetitions from some term, then for each term there is a number of repetition that maps the term to itself. Intuitively this holds by a pigeonhole principle: If for each term you need to pick a term from that you can reach it, but only finitely many terms are available, then eventually you need to complete a cycle. -/
+theorem repeat_each_reaches_self_of_each_reachable
+    (h : GroundTermMapping sig)
+    (ts : List (GroundTerm sig))
+    (each_reachable : ∀ t, t ∈ ts -> ∃ k, 1 ≤ k ∧ ∃ s, s ∈ ts ∧ (h.repeat_hom k) s = t) :
+    (∀ s, s ∈ ts -> ∃ l, 1 ≤ l ∧ (h.repeat_hom l) s = s) := by
+  induction ts with
+  | nil => simp
+  | cons hd tl ih =>
+    specialize ih (by
       intro t t_mem
-      exists 1
-      constructor
-      . simp
-      . simp only [repeat_hom]
-        apply surj t t_mem
+      have each_reachable_for_t := each_reachable t (by simp [t_mem])
+      rcases each_reachable_for_t with ⟨k, k_le, s, s_mem, s_eq⟩
+      simp only [List.mem_cons] at s_mem
+      cases s_mem with
+      | inr s_mem => exists k; constructor; exact k_le; exists s
+      | inl s_mem =>
+        have each_reachable_for_s := each_reachable s (by simp [s_mem])
+        rcases each_reachable_for_s with ⟨l, l_le, u, u_mem, u_eq⟩
+        simp only [List.mem_cons] at u_mem
+        cases u_mem with
+        | inl u_mem =>
+          exists (((k / l) + 1) * l)
+          constructor
+          .
+            rw [Nat.add_mul]
+            apply Nat.le_trans
+            . exact k_le
+            . apply Nat.le_of_lt
+              simp
+              -- NOTE: taken from https://github.com/leanprover-community/mathlib4/blob/3f813de52d8cffaa73e27edd62364eec90eac633/Mathlib/Data/Nat/Defs.lean#L473-L474
+              rw [← Nat.succ_mul, ← Nat.div_lt_iff_lt_mul (by apply Nat.lt_of_succ_le; exact l_le)]; exact Nat.lt_succ_self _
+          . exists t
+            constructor
+            . exact t_mem
+            . apply h.repeat_hom_move_cycle s
+              . rw [Nat.mul_comm]
+                apply h.repeat_hom_cycle_mul
+                rw [u_mem, ← s_mem] at u_eq
+                exact u_eq
+              . exact s_eq
+        | inr u_mem =>
+          exists (k + l)
+          constructor
+          . apply Nat.le_add_right_of_le; exact k_le
+          . exists u
+            constructor
+            . exact u_mem
+            . rw [GroundTermMapping.repeat_hom_add]
+              rw [u_eq, s_eq]
     )
-    have repeats_globally := h.repeat_globally_of_each_repeats ts each_repeats
 
-    rcases repeats_globally with ⟨k, le, repeats_globally⟩
+    intro s s_mem
+    simp only [List.mem_cons] at s_mem
+    cases s_mem with
+    | inl s_mem =>
+      specialize each_reachable s (by rw [s_mem]; simp)
+      rcases each_reachable with ⟨k, k_le, t, t_mem, t_eq⟩
+      simp only [List.mem_cons] at t_mem
+      cases t_mem with
+      | inl t_mem => exists k; constructor; exact k_le; rw [t_mem, ← s_mem] at t_eq; exact t_eq
+      | inr t_mem =>
+        specialize ih t t_mem
+        rcases ih with ⟨l, l_le, ih⟩
+        exists l
+        constructor
+        . exact l_le
+        . apply h.repeat_hom_move_cycle t
+          . exact ih
+          . exact t_eq
+    | inr s_mem =>
+      apply ih
+      exact s_mem
 
-    exists k-1
-    intro t t_mem
-    have repeat_add := h.repeat_hom_add (k-1) 1 t
-    conv at repeat_add => right; right; simp [repeat_hom]
-    rw [← repeat_add]
-    rw [Nat.sub_one_add_one]
-    . apply repeats_globally; exact t_mem
-    . apply Nat.ne_zero_of_lt; apply Nat.lt_of_succ_le; exact le
-
-  theorem repeat_hom_id_on_const (h : GroundTermMapping sig) (idOnConst : h.isIdOnConstants) : ∀ i, (h.repeat_hom i).isIdOnConstants := by
-    intro i
-    induction i with
-    | zero => unfold repeat_hom; intro c; simp
-    | succ i ih =>
-      intro c
-      unfold repeat_hom
-      rw [Function.comp_apply, ih, idOnConst]
-
-  variable [DecidableEq sig.P]
-
-  theorem repeat_hom_isHomomorphism (h : GroundTermMapping sig) (fs : FactSet sig) (hom : h.isHomomorphism fs fs) : ∀ i, (h.repeat_hom i).isHomomorphism fs fs := by
-    intro i
+/-- If each term from a finite list is mapped to itself after some number of repetitions, then there is a global repetition number that maps each term to itself. Basically any common multiple of the individual repetition numbers works. -/
+theorem repeat_globally_of_each_repeats
+    (h : GroundTermMapping sig)
+    (ts : List (GroundTerm sig))
+    (each_repeats : ∀ s, s ∈ ts -> ∃ l, 1 ≤ l ∧ (h.repeat_hom l) s = s) :
+    ∃ l, 1 ≤ l ∧ ∀ s, s ∈ ts -> (h.repeat_hom l) s = s := by
+  induction ts with
+  | nil => exists 1; simp
+  | cons hd tl ih =>
+    specialize ih (by intro s s_mem; apply each_repeats; simp [s_mem])
+    rcases ih with ⟨l_ih, l_ih_le, ih⟩
+    rcases each_repeats hd (by simp) with ⟨l_hd, l_hd_le, each_repeats⟩
+    exists l_hd * l_ih
     constructor
-    . apply repeat_hom_id_on_const; exact hom.left
-    . induction i with
-      | zero =>
-        simp [repeat_hom]
-        intro f f_mem
-        rcases f_mem with ⟨f', f'_mem, f_eq⟩
-        have : f = f' := by
-          unfold TermMapping.apply_generalized_atom at f_eq
-          rw [f_eq]; simp
-        rw [this]
-        exact f'_mem
-      | succ i ih =>
-        unfold repeat_hom
-        unfold applyFactSet
-        rw [TermMapping.apply_generalized_atom_set_compose, Function.comp_apply]
-        intro f f_mem
-        apply hom.right
-        apply h.apply_generalized_atom_set_subset_of_subset
-        . exact ih
-        . exact f_mem
+    . apply Nat.le_trans; exact l_hd_le; apply Nat.le_mul_of_pos_right; apply Nat.lt_of_succ_le; exact l_ih_le
+    . intro s s_mem
+      simp only [List.mem_cons] at s_mem
+      cases s_mem with
+      | inl s_mem => rw [s_mem, h.repeat_hom_cycle_mul]; exact each_repeats
+      | inr s_mem => specialize ih s s_mem; rw [Nat.mul_comm, h.repeat_hom_cycle_mul]; exact ih
+
+/-- If a mapping is surjective for a given list of terms, then there exists a repetition count $k$ such that $k+1$ map each term from the list to itself. Note that we use $k+1$ repetitions as otherwise the result would be trivial for zero repetitions, which are the id by definition. -/
+theorem exists_repetition_that_is_inverse_of_surj (h : GroundTermMapping sig) (ts : List (GroundTerm sig)) (surj : h.surjective_for_domain_and_image_list ts ts) : ∃ k, ∀ t, t ∈ ts -> (h.repeat_hom k) (h t) = t := by
+  have each_repeats := h.repeat_each_reaches_self_of_each_reachable ts (by
+    intro t t_mem
+    exists 1
+    constructor
+    . simp
+    . simp only [repeat_hom]
+      apply surj t t_mem
+  )
+  have repeats_globally := h.repeat_globally_of_each_repeats ts each_repeats
+
+  rcases repeats_globally with ⟨k, le, repeats_globally⟩
+
+  exists k-1
+  intro t t_mem
+  have repeat_add := h.repeat_hom_add (k-1) 1 t
+  conv at repeat_add => right; right; simp [repeat_hom]
+  rw [← repeat_add]
+  rw [Nat.sub_one_add_one]
+  . apply repeats_globally; exact t_mem
+  . apply Nat.ne_zero_of_lt; apply Nat.lt_of_succ_le; exact le
+
+/-- Repeating a mapping retains the `isIdOnConstants` property. -/
+theorem repeat_hom_id_on_const (h : GroundTermMapping sig) (idOnConst : h.isIdOnConstants) : ∀ i, (h.repeat_hom i).isIdOnConstants := by
+  intro i
+  induction i with
+  | zero => unfold repeat_hom; intro c; simp
+  | succ i ih =>
+    intro c
+    unfold repeat_hom
+    rw [Function.comp_apply, ih, idOnConst]
+
+variable [DecidableEq sig.P]
+
+/-- Repeating a mapping retains the `isHomomorphism` property at least for endomorphisms. -/
+theorem repeat_hom_isHomomorphism (h : GroundTermMapping sig) (fs : FactSet sig) (hom : h.isHomomorphism fs fs) : ∀ i, (h.repeat_hom i).isHomomorphism fs fs := by
+  intro i
+  constructor
+  . apply repeat_hom_id_on_const; exact hom.left
+  . induction i with
+    | zero =>
+      simp only [repeat_hom]
+      intro f f_mem
+      rcases f_mem with ⟨f', f'_mem, f_eq⟩
+      have : f = f' := by
+        unfold TermMapping.apply_generalized_atom at f_eq
+        rw [f_eq]; simp
+      rw [this]
+      exact f'_mem
+    | succ i ih =>
+      unfold repeat_hom
+      unfold applyFactSet
+      rw [TermMapping.apply_generalized_atom_set_compose, Function.comp_apply]
+      intro f f_mem
+      apply hom.right
+      apply h.apply_generalized_atom_set_subset_of_subset
+      . exact ih
+      . exact f_mem
 
 end GroundTermMapping
 
-end HomomorphismRepetition
-
-
 namespace FactSet
 
-  variable {sig : Signature} [DecidableEq sig.P] [DecidableEq sig.C] [DecidableEq sig.V]
+/-!
+## Cores Definitions and some of their Properties
 
-  def isWeakCore (fs : FactSet sig) : Prop :=
-    ∀ (h : GroundTermMapping sig), h.isHomomorphism fs fs -> h.strong fs.terms fs fs ∧ h.injective_for_domain_set fs.terms
+Here, we finally define `isWeakCore` and `isStrongCore` and show some of their relations and additional properties. This also involves some more theorems about homomorphisms.
+-/
 
-  def isStrongCore (fs : FactSet sig) : Prop :=
-    ∀ (h : GroundTermMapping sig), h.isHomomorphism fs fs -> h.strong fs.terms fs fs ∧ h.injective_for_domain_set fs.terms ∧ h.surjective_for_domain_and_image_set fs.terms fs.terms
+variable {sig : Signature} [DecidableEq sig.P] [DecidableEq sig.C] [DecidableEq sig.V]
 
-  def homSubset (c fs : FactSet sig) : Prop := c ⊆ fs ∧ (∃ (h : GroundTermMapping sig), h.isHomomorphism fs c)
+/-- A `FactSet` is a weak core if every endomorphisms on the fact set is strong and injective. -/
+def isWeakCore (fs : FactSet sig) : Prop :=
+  ∀ (h : GroundTermMapping sig), h.isHomomorphism fs fs -> h.strong fs.terms fs fs ∧ h.injective_for_domain_set fs.terms
 
-  theorem hom_surjective_of_finite_of_injective (fs : FactSet sig) (finite : fs.finite) : ∀ (h : GroundTermMapping sig), h.isHomomorphism fs fs -> h.injective_for_domain_set fs.terms -> h.surjective_for_domain_and_image_set fs.terms fs.terms := by
-    rcases finite with ⟨l, finite⟩
-    intro h isHom inj
+/-- A `FactSet` is a strong core if every endomorphisms on the fact set is strong, injective, and surjective. (By definition, every strong core is a weak core.) -/
+def isStrongCore (fs : FactSet sig) : Prop :=
+  ∀ (h : GroundTermMapping sig), h.isHomomorphism fs fs -> h.strong fs.terms fs fs ∧ h.injective_for_domain_set fs.terms ∧ h.surjective_for_domain_and_image_set fs.terms fs.terms
 
-    let terms_list := (l.map GeneralizedAtom.terms).flatten.eraseDupsKeepRight
-    have nodup_terms_list : terms_list.Nodup := by apply List.nodup_eraseDupsKeepRight
-    have mem_terms_list : ∀ e, e ∈ terms_list ↔ e ∈ fs.terms := by
-      simp only [terms_list]
-      intro e
-      rw [List.mem_eraseDupsKeepRight]
-      unfold FactSet.terms
-      simp
+/-- We say that a fact set $C$ is a homomorphic subset of another fact set $F$ if $C$ is a subset of $F$ and there is a homomorphism from $F$ to $C$. -/
+def homSubset (c fs : FactSet sig) : Prop := c ⊆ fs ∧ (∃ (h : GroundTermMapping sig), h.isHomomorphism fs c)
+
+/-- For a homomorphism on a finite fact set, injectivity implies surjectivity. -/
+theorem hom_surjective_of_finite_of_injective (fs : FactSet sig) (finite : fs.finite) : ∀ (h : GroundTermMapping sig), h.isHomomorphism fs fs -> h.injective_for_domain_set fs.terms -> h.surjective_for_domain_and_image_set fs.terms fs.terms := by
+  rcases finite with ⟨l, finite⟩
+  intro h isHom inj
+
+  let terms_list := (l.map GeneralizedAtom.terms).flatten.eraseDupsKeepRight
+  have nodup_terms_list : terms_list.Nodup := by apply List.nodup_eraseDupsKeepRight
+  have mem_terms_list : ∀ e, e ∈ terms_list ↔ e ∈ fs.terms := by
+    simp only [terms_list]
+    intro e
+    rw [List.mem_eraseDupsKeepRight]
+    unfold FactSet.terms
+    simp only [List.mem_flatten, List.mem_map]
+    constructor
+    . intro h
+      rcases h with ⟨ts, h, ts_mem⟩
+      rcases h with ⟨f, f_mem, eq⟩
+      exists f
+      rw [eq]
+      rw [← finite.right f]
+      constructor <;> assumption
+    . intro h
+      rcases h with ⟨f, f_mem, e_mem⟩
+      exists f.terms
       constructor
-      . intro h
-        rcases h with ⟨ts, h, ts_mem⟩
-        rcases h with ⟨f, f_mem, eq⟩
-        exists f
-        rw [eq]
-        rw [← finite.right f]
-        constructor <;> assumption
-      . intro h
-        rcases h with ⟨f, f_mem, e_mem⟩
-        exists f.terms
-        constructor
-        . exists f; rw [finite.right f]; constructor; exact f_mem; rfl
-        . exact e_mem
-    have closed : ∀ e, e ∈ terms_list -> h e ∈ terms_list := by
-      simp only [terms_list]
-      intro e
-      rw [List.mem_eraseDupsKeepRight]
-      rw [List.mem_eraseDupsKeepRight]
-      simp
-      intro f f_mem e_in_f
-      let f' := h.applyFact f
-      have f'_mem : f' ∈ fs := by
-        apply isHom.right
-        unfold GroundTermMapping.applyFactSet
-        exists f
-        constructor
-        . rw [finite.right] at f_mem
-          exact f_mem
-        . rfl
-      exists f'.terms
+      . exists f; rw [finite.right f]; constructor; exact f_mem; rfl
+      . exact e_mem
+  have closed : ∀ e, e ∈ terms_list -> h e ∈ terms_list := by
+    simp only [terms_list]
+    intro e
+    rw [List.mem_eraseDupsKeepRight]
+    rw [List.mem_eraseDupsKeepRight]
+    simp only [List.mem_flatten, List.mem_map, forall_exists_index, and_imp, forall_apply_eq_imp_iff₂]
+    intro f f_mem e_in_f
+    let f' := h.applyFact f
+    have f'_mem : f' ∈ fs := by
+      apply isHom.right
+      unfold GroundTermMapping.applyFactSet
+      exists f
       constructor
-      . exists f'
-        constructor
-        . rw [finite.right]; exact f'_mem
-        . rfl
-      . simp only [f', TermMapping.apply_generalized_atom]
+      . rw [finite.right] at f_mem
+        exact f_mem
+      . rfl
+    exists f'.terms
+    constructor
+    . exists f'
+      constructor
+      . rw [finite.right]; exact f'_mem
+      . rfl
+    . simp only [f', TermMapping.apply_generalized_atom]
+      rw [List.mem_map]
+      exists e
+
+  rw [Function.surjective_set_list_equiv h fs.terms terms_list mem_terms_list fs.terms terms_list mem_terms_list]
+  rw [← Function.injective_iff_surjective_of_nodup_of_closed h terms_list nodup_terms_list closed]
+  rw [← Function.injective_set_list_equiv h fs.terms terms_list mem_terms_list]
+  exact inj
+
+/-- For a homomorphism on a finite fact set, injectivity implies that the homomorphisms is also strong. -/
+theorem hom_strong_of_finite_of_injective (fs : FactSet sig) (finite : fs.finite) : ∀ (h : GroundTermMapping sig), h.isHomomorphism fs fs -> h.injective_for_domain_set fs.terms -> h.strong fs.terms fs fs := by
+  intro h isHom inj
+
+  intro f ts_mem f_not_mem apply_mem
+  apply f_not_mem
+
+  have surj := fs.hom_surjective_of_finite_of_injective finite h isHom inj
+
+  have terms_finite := fs.terms_finite_of_finite finite
+  rcases terms_finite with ⟨terms, nodup, equiv⟩
+
+  rw [h.surjective_set_list_equiv fs.terms terms equiv fs.terms terms equiv] at surj
+  have ex_inv := h.exists_repetition_that_is_inverse_of_surj terms surj
+  rcases ex_inv with ⟨k, inv⟩
+  have inv_hom : (h.repeat_hom k).isHomomorphism fs fs := h.repeat_hom_isHomomorphism fs isHom k
+
+  have : (h.repeat_hom k).applyFact (h.applyFact f) = f := by
+    unfold GroundTermMapping.applyFact
+    rw [← TermMapping.apply_generalized_atom_compose']
+    apply TermMapping.apply_generalized_atom_eq_self_of_id_on_terms
+    intro t t_mem
+    rw [Function.comp_apply]
+    apply inv
+    rw [equiv]
+    apply ts_mem
+    exact t_mem
+  rw [← this]
+
+  apply inv_hom.right
+  apply TermMapping.apply_generalized_atom_mem_apply_generalized_atom_set
+  exact apply_mem
+
+/-- For finite fact sets, `isWeakCore` implies `isStrongCore`. That means that `isWeakCore` and `isStrongCore` are equivalent on finite fact sets. -/
+theorem isStrongCore_of_isWeakCore_of_finite (fs : FactSet sig) (weakCore : fs.isWeakCore) (finite : fs.finite) : fs.isStrongCore := by
+  rcases finite with ⟨l, finite⟩
+  unfold isStrongCore
+  intro h isHom
+  specialize weakCore h isHom
+  rcases weakCore with ⟨strong, injective⟩
+  constructor
+  . exact strong
+  constructor
+  . exact injective
+  . apply hom_surjective_of_finite_of_injective
+    . unfold Set.finite; exists l
+    . exact isHom
+    . exact injective
+
+/-- Given two fact sets A,B of which one is a weak and one is a strong core, if there are homomorphisms from A to B and B to A, then there exists an isomorphism from A to B, i.e. a strong homomorphisms that is injective and surjective. -/
+theorem every_weakCore_isomorphic_to_strongCore_of_hom_both_ways
+    (sc : FactSet sig) (sc_strong : sc.isStrongCore)
+    (wc : FactSet sig) (wc_weak : wc.isWeakCore)
+    (h_sc_wc h_wc_sc : GroundTermMapping sig) (h_sc_wc_hom : h_sc_wc.isHomomorphism sc wc) (h_wc_sc_hom : h_wc_sc.isHomomorphism wc sc) :
+    ∃ (iso : GroundTermMapping sig), iso.isHomomorphism wc sc ∧ iso.strong wc.terms wc sc ∧ iso.injective_for_domain_set wc.terms ∧ iso.surjective_for_domain_and_image_set wc.terms sc.terms := by
+
+  specialize wc_weak (h_sc_wc ∘ h_wc_sc) (by
+    apply GroundTermMapping.isHomomorphism_compose
+    . exact h_wc_sc_hom
+    . exact h_sc_wc_hom
+  )
+
+  specialize sc_strong (h_wc_sc ∘ h_sc_wc) (by
+    apply GroundTermMapping.isHomomorphism_compose
+    . exact h_sc_wc_hom
+    . exact h_wc_sc_hom
+  )
+
+  exists h_wc_sc
+  constructor
+  . exact h_wc_sc_hom
+  constructor
+  -- strong since h_sc_wc ∘ h_wc_sc is strong
+  . apply GroundTermMapping.strong_of_compose_strong h_wc_sc h_sc_wc wc.terms wc sc wc h_sc_wc_hom
+    exact wc_weak.left
+  constructor
+  -- injective since h_sc_wc ∘ h_wc_sc is injective
+  . apply Function.injective_of_injective_compose h_wc_sc h_sc_wc
+    exact wc_weak.right
+  -- surjective since h_wc_sc ∘ h_sc_wc is surjective
+  . apply Function.surjective_of_surjective_from_subset
+    . apply Function.surjective_of_surjective_compose h_sc_wc h_wc_sc sc.terms
+      exact sc_strong.right.right
+    . intro t t_mem_image
+      rcases t_mem_image with ⟨arg, arg_mem, arg_eq⟩
+      rcases arg_mem with ⟨f, f_mem, f_eq⟩
+      exists (h_sc_wc.applyFact f)
+      constructor
+      . apply h_sc_wc_hom.right
+        exists f
+      . unfold GroundTermMapping.applyFact
+        unfold TermMapping.apply_generalized_atom
         rw [List.mem_map]
-        exists e
+        exists arg; simp [f_eq, arg_eq]
 
-    rw [Function.surjective_set_list_equiv h fs.terms terms_list mem_terms_list fs.terms terms_list mem_terms_list]
-    rw [← Function.injective_iff_surjective_of_nodup_of_closed h terms_list nodup_terms_list closed]
-    rw [← Function.injective_set_list_equiv h fs.terms terms_list mem_terms_list]
-    exact inj
+/-- Strong cores of fact sets are unique up to isomorphism. That is, consider a fact set $F$. A strong core $C$ for $F$ is a strong core that is also a homomorphic subset of $F$. Now every (other) homomorphic subset $C'$ of $F$ that is at least a weak core has an isomorphism into $C$. -/
+theorem strongCore_unique_up_to_isomorphism_with_respect_to_weak_cores
+    (fs : FactSet sig)
+    (sc : FactSet sig) (sub_sc : sc.homSubset fs) (sc_strong : sc.isStrongCore)
+    (wc : FactSet sig) (sub_wc : wc.homSubset fs) (wc_weak : wc.isWeakCore) :
+    ∃ (iso : GroundTermMapping sig), iso.isHomomorphism wc sc ∧ iso.strong wc.terms wc sc ∧ iso.injective_for_domain_set wc.terms ∧ iso.surjective_for_domain_and_image_set wc.terms sc.terms := by
 
-  theorem hom_strong_of_finite_of_injective (fs : FactSet sig) (finite : fs.finite) : ∀ (h : GroundTermMapping sig), h.isHomomorphism fs fs -> h.injective_for_domain_set fs.terms -> h.strong fs.terms fs fs := by
-    intro h isHom inj
+  rcases sub_sc with ⟨sub_sc, h_fs_sc, h_fs_sc_hom⟩
+  rcases sub_wc with ⟨sub_wc, h_fs_wc, h_fs_wc_hom⟩
 
-    intro f ts_mem f_not_mem apply_mem
-    apply f_not_mem
+  have h_sc_wc_hom : h_fs_wc.isHomomorphism sc wc := by
+    constructor
+    . exact h_fs_wc_hom.left
+    . apply Set.subset_trans (b := h_fs_wc.applyFactSet fs)
+      . apply TermMapping.apply_generalized_atom_set_subset_of_subset
+        exact sub_sc
+      . exact h_fs_wc_hom.right
 
-    have surj := fs.hom_surjective_of_finite_of_injective finite h isHom inj
+  have h_wc_sc_hom : h_fs_sc.isHomomorphism wc sc := by
+    constructor
+    . exact h_fs_sc_hom.left
+    . apply Set.subset_trans (b := h_fs_sc.applyFactSet fs)
+      . apply TermMapping.apply_generalized_atom_set_subset_of_subset
+        exact sub_wc
+      . exact h_fs_sc_hom.right
 
-    have terms_finite := fs.terms_finite_of_finite finite
-    rcases terms_finite with ⟨terms, nodup, equiv⟩
+  exact every_weakCore_isomorphic_to_strongCore_of_hom_both_ways sc sc_strong wc wc_weak h_fs_wc h_fs_sc h_sc_wc_hom h_wc_sc_hom
 
-    rw [h.surjective_set_list_equiv fs.terms terms equiv fs.terms terms equiv] at surj
-    have ex_inv := h.exists_repetition_that_is_inverse_of_surj terms surj
-    rcases ex_inv with ⟨k, inv⟩
-    have inv_hom : (h.repeat_hom k).isHomomorphism fs fs := h.repeat_hom_isHomomorphism fs isHom k
+/-- Consider a `KnowledgeBase` and a universal model of the KB that is a strong core. Then every (other) universal model that is at least a weak core, is isomorphism to the strong core. -/
+theorem every_universal_weakCore_isomorphic_to_universal_strongCore
+    {kb : KnowledgeBase sig}
+    (sc : FactSet sig) (sc_universal : sc.universallyModelsKb kb) (sc_strong : sc.isStrongCore)
+    (wc : FactSet sig) (wc_universal : wc.universallyModelsKb kb) (wc_weak : wc.isWeakCore) :
+    ∃ (iso : GroundTermMapping sig), iso.isHomomorphism wc sc ∧ iso.strong wc.terms wc sc ∧ iso.injective_for_domain_set wc.terms ∧ iso.surjective_for_domain_and_image_set wc.terms sc.terms := by
 
-    have : (h.repeat_hom k).applyFact (h.applyFact f) = f := by
-      unfold GroundTermMapping.applyFact
-      rw [← TermMapping.apply_generalized_atom_compose']
+  rcases sc_universal.right wc wc_universal.left with ⟨h_sc_wc, h_sc_wc_hom⟩
+  rcases wc_universal.right sc sc_universal.left with ⟨h_wc_sc, h_wc_sc_hom⟩
+
+  exact every_weakCore_isomorphic_to_strongCore_of_hom_both_ways sc sc_strong wc wc_weak h_sc_wc h_wc_sc h_sc_wc_hom h_wc_sc_hom
+
+/-- Given a model of a `KnowledgeBase`, every strong core of the model is also a model. In general, this does *not* hold for weak cores (in the infinite setting). -/
+theorem strong_core_of_model_is_model
+    {kb : KnowledgeBase sig}
+    (fs : FactSet sig) (fs_model : fs.modelsKb kb)
+    (sc : FactSet sig) (sc_sub : sc.homSubset fs) (sc_strong : sc.isStrongCore) :
+    sc.modelsKb kb := by
+
+  rcases sc_sub with ⟨sc_sub, h_fs_sc, h_fs_sc_hom⟩
+
+  have h_fs_sc_endo_sc : h_fs_sc.isHomomorphism sc sc := by
+    constructor
+    . exact h_fs_sc_hom.left
+    . apply Set.subset_trans (b := h_fs_sc.applyFactSet fs)
+      . apply TermMapping.apply_generalized_atom_set_subset_of_subset
+        exact sc_sub
+      . exact h_fs_sc_hom.right
+
+  specialize sc_strong h_fs_sc h_fs_sc_endo_sc
+
+  -- TODO: extract this into a general result; check which properties we really need and want here
+  have ex_inv : ∃ (inv : GroundTermMapping sig), (∀ t, t ∈ sc.terms -> (h_fs_sc (inv t)) = t) ∧ inv.isHomomorphism sc sc := by
+    let inv : GroundTermMapping sig := fun t =>
+      have dev := Classical.propDecidable (t ∈ sc.terms)
+      if t_mem : t ∈ sc.terms
+      then
+        Classical.choose (sc_strong.right.right t t_mem)
+      else
+        t
+
+    have inv_id : (∀ t, t ∈ sc.terms -> (h_fs_sc (inv t)) = t) := by
+      intro t t_mem
+      unfold inv
+      simp only [t_mem, ↓reduceDIte]
+      have spec := Classical.choose_spec (sc_strong.right.right t t_mem)
+      exact spec.right
+    exists inv
+
+    constructor
+    . exact inv_id
+    . constructor
+      . intro c
+        unfold inv
+        cases Classical.em (GroundTerm.const c ∈ sc.terms) with
+        | inr n_mem => simp [n_mem]
+        | inl mem =>
+          simp only [mem, ↓reduceDIte]
+          have spec := Classical.choose_spec (sc_strong.right.right (GroundTerm.const c) mem)
+          apply sc_strong.right.left
+          . exact spec.left
+          . exact mem
+          . rw [spec.right, h_fs_sc_hom.left]
+      . intro f f_mem
+        rcases f_mem with ⟨f', f'_mem, f_eq⟩
+        have strong := sc_strong.left
+        unfold GroundTermMapping.strong at strong
+        apply Classical.byContradiction
+        intro contra
+        apply strong f
+        . intro t t_mem
+          rw [f_eq] at t_mem
+          unfold TermMapping.apply_generalized_atom at t_mem
+          rw [List.mem_map] at t_mem
+          rcases t_mem with ⟨t', t'_mem, t_eq⟩
+          have t'_mem : t' ∈ sc.terms := by exists f'
+          have spec := Classical.choose_spec (sc_strong.right.right t' t'_mem)
+          rw [← t_eq]
+          unfold inv
+          simp only [t'_mem, ↓reduceDIte]
+          exact spec.left
+        . exact contra
+        . rw [f_eq]
+          unfold GroundTermMapping.applyFact
+          rw [← TermMapping.apply_generalized_atom_compose']
+          have : TermMapping.apply_generalized_atom (h_fs_sc ∘ inv) f' = f' := by
+            apply TermMapping.apply_generalized_atom_eq_self_of_id_on_terms
+            intro t t_mem
+            rw [Function.comp_apply, inv_id]
+            exists f'
+          rw [this]
+          exact f'_mem
+  rcases ex_inv with ⟨inv, inv_id, inv_hom⟩
+
+  constructor
+  . intro f f_mem
+    have : h_fs_sc.applyFact f = f := by
+      have prop := kb.db.toFactSet.property.right
+      unfold FactSet.isFunctionFree at prop
+      unfold Fact.isFunctionFree at prop
+      specialize prop f f_mem
       apply TermMapping.apply_generalized_atom_eq_self_of_id_on_terms
       intro t t_mem
-      rw [Function.comp_apply]
-      apply inv
-      rw [equiv]
-      apply ts_mem
-      exact t_mem
+      rcases (prop t t_mem) with ⟨c, t_eq⟩
+      rw [t_eq]
+      exact h_fs_sc_hom.left
     rw [← this]
-
-    apply inv_hom.right
+    apply h_fs_sc_hom.right
     apply TermMapping.apply_generalized_atom_mem_apply_generalized_atom_set
-    exact apply_mem
+    apply fs_model.left
+    exact f_mem
+  . intro r r_mem
+    intro subs loaded
 
-  theorem isStrongCore_of_isWeakCore_of_finite (fs : FactSet sig) (weakCore : fs.isWeakCore) (finite : fs.finite) : fs.isStrongCore := by
-    rcases finite with ⟨l, finite⟩
-    unfold isStrongCore
-    intro h isHom
-    specialize weakCore h isHom
-    rcases weakCore with ⟨strong, injective⟩
-    constructor
-    . exact strong
-    constructor
-    . exact injective
-    . apply hom_surjective_of_finite_of_injective
-      . unfold Set.finite; exists l
-      . exact isHom
-      . exact injective
-
-  theorem every_weakCore_isomorphic_to_strongCore_of_hom_both_ways
-      (sc : FactSet sig) (sc_strong : sc.isStrongCore)
-      (wc : FactSet sig) (wc_weak : wc.isWeakCore)
-      (h_sc_wc h_wc_sc : GroundTermMapping sig) (h_sc_wc_hom : h_sc_wc.isHomomorphism sc wc) (h_wc_sc_hom : h_wc_sc.isHomomorphism wc sc) :
-      ∃ (iso : GroundTermMapping sig), iso.isHomomorphism wc sc ∧ iso.strong wc.terms wc sc ∧ iso.injective_for_domain_set wc.terms ∧ iso.surjective_for_domain_and_image_set wc.terms sc.terms := by
-
-    specialize wc_weak (h_sc_wc ∘ h_wc_sc) (by
-      apply GroundTermMapping.isHomomorphism_compose
-      . exact h_wc_sc_hom
-      . exact h_sc_wc_hom
+    have fs_models_rule := fs_model.right r r_mem (inv ∘ subs)
+    specialize fs_models_rule (by
+      apply Set.subset_trans (b := inv.applyFactSet sc)
+      . intro f f_mem
+        unfold GroundSubstitution.apply_function_free_conj at f_mem
+        unfold TermMapping.apply_generalized_atom_list at f_mem
+        rw [List.mem_toSet, List.mem_map] at f_mem
+        rcases f_mem with ⟨a, a_mem, f_eq⟩
+        rw [← GroundSubstitution.apply_function_free_atom.eq_def, GroundSubstitution.apply_function_free_atom_compose_of_isIdOnConstants _ _ inv_hom.left] at f_eq
+        rw [← f_eq]
+        apply TermMapping.apply_generalized_atom_mem_apply_generalized_atom_set
+        apply loaded
+        unfold GroundSubstitution.apply_function_free_conj
+        unfold TermMapping.apply_generalized_atom_list
+        rw [List.mem_toSet, List.mem_map]
+        exists a
+      . apply Set.subset_trans (b := sc)
+        . exact inv_hom.right
+        . exact sc_sub
     )
+    rcases fs_models_rule with ⟨i, subs', frontier_mapping, sub_mapping⟩
 
-    specialize sc_strong (h_wc_sc ∘ h_sc_wc) (by
-      apply GroundTermMapping.isHomomorphism_compose
-      . exact h_sc_wc_hom
-      . exact h_wc_sc_hom
-    )
-
-    exists h_wc_sc
+    exists i
+    exists (h_fs_sc ∘ subs')
     constructor
-    . exact h_wc_sc_hom
-    constructor
-    -- strong since h_sc_wc ∘ h_wc_sc is strong
-    . apply GroundTermMapping.strong_of_compose_strong h_wc_sc h_sc_wc wc.terms wc sc wc h_sc_wc_hom
-      exact wc_weak.left
-    constructor
-    -- injective since h_sc_wc ∘ h_wc_sc is injective
-    . apply Function.injective_of_injective_compose h_wc_sc h_sc_wc
-      exact wc_weak.right
-    -- surjective since h_wc_sc ∘ h_sc_wc is surjective
-    . apply Function.surjective_of_surjective_from_subset
-      . apply Function.surjective_of_surjective_compose h_sc_wc h_wc_sc sc.terms
-        exact sc_strong.right.right
-      . intro t t_mem_image
-        rcases t_mem_image with ⟨arg, arg_mem, arg_eq⟩
-        rcases arg_mem with ⟨f, f_mem, f_eq⟩
-        exists (h_sc_wc.applyFact f)
+    . intro v v_mem
+      rw [Function.comp_apply]
+      rw [frontier_mapping v v_mem]
+      rw [Function.comp_apply]
+      rw [inv_id _ (by
+        unfold Rule.frontier at v_mem
+        rw [List.mem_filter] at v_mem
+        have v_mem := v_mem.left
+        unfold FunctionFreeConjunction.vars at v_mem
+        rw [List.mem_flatMap] at v_mem
+        rcases v_mem with ⟨a, a_mem, v_mem⟩
+        exists subs.apply_function_free_atom a
         constructor
-        . apply h_sc_wc_hom.right
-          exists f
-        . unfold GroundTermMapping.applyFact
+        . apply loaded
+          unfold GroundSubstitution.apply_function_free_conj
+          unfold TermMapping.apply_generalized_atom_list
+          rw [List.mem_toSet, List.mem_map]
+          exists a
+        . unfold GroundSubstitution.apply_function_free_atom
           unfold TermMapping.apply_generalized_atom
           rw [List.mem_map]
-          exists arg
-
-  theorem strongCore_unique_up_to_isomorphism_with_respect_to_weak_cores
-      (fs : FactSet sig)
-      (sc : FactSet sig) (sub_sc : sc.homSubset fs) (sc_strong : sc.isStrongCore)
-      (wc : FactSet sig) (sub_wc : wc.homSubset fs) (wc_weak : wc.isWeakCore) :
-      ∃ (iso : GroundTermMapping sig), iso.isHomomorphism wc sc ∧ iso.strong wc.terms wc sc ∧ iso.injective_for_domain_set wc.terms ∧ iso.surjective_for_domain_and_image_set wc.terms sc.terms := by
-
-    rcases sub_sc with ⟨sub_sc, h_fs_sc, h_fs_sc_hom⟩
-    rcases sub_wc with ⟨sub_wc, h_fs_wc, h_fs_wc_hom⟩
-
-    have h_sc_wc_hom : h_fs_wc.isHomomorphism sc wc := by
-      constructor
-      . exact h_fs_wc_hom.left
-      . apply Set.subset_trans (b := h_fs_wc.applyFactSet fs)
-        . apply TermMapping.apply_generalized_atom_set_subset_of_subset
-          exact sub_sc
-        . exact h_fs_wc_hom.right
-
-    have h_wc_sc_hom : h_fs_sc.isHomomorphism wc sc := by
-      constructor
-      . exact h_fs_sc_hom.left
-      . apply Set.subset_trans (b := h_fs_sc.applyFactSet fs)
-        . apply TermMapping.apply_generalized_atom_set_subset_of_subset
-          exact sub_wc
-        . exact h_fs_sc_hom.right
-
-    exact every_weakCore_isomorphic_to_strongCore_of_hom_both_ways sc sc_strong wc wc_weak h_fs_wc h_fs_sc h_sc_wc_hom h_wc_sc_hom
-
-  theorem every_universal_weakCore_isomorphic_to_universal_strongCore
-      {kb : KnowledgeBase sig}
-      (sc : FactSet sig) (sc_universal : sc.universallyModelsKb kb) (sc_strong : sc.isStrongCore)
-      (wc : FactSet sig) (wc_universal : wc.universallyModelsKb kb) (wc_weak : wc.isWeakCore) :
-      ∃ (iso : GroundTermMapping sig), iso.isHomomorphism wc sc ∧ iso.strong wc.terms wc sc ∧ iso.injective_for_domain_set wc.terms ∧ iso.surjective_for_domain_and_image_set wc.terms sc.terms := by
-
-    rcases sc_universal.right wc wc_universal.left with ⟨h_sc_wc, h_sc_wc_hom⟩
-    rcases wc_universal.right sc sc_universal.left with ⟨h_wc_sc, h_wc_sc_hom⟩
-
-    exact every_weakCore_isomorphic_to_strongCore_of_hom_both_ways sc sc_strong wc wc_weak h_sc_wc h_wc_sc h_sc_wc_hom h_wc_sc_hom
-
-  theorem strong_core_of_model_is_model
-      {kb : KnowledgeBase sig}
-      (fs : FactSet sig) (fs_model : fs.modelsKb kb)
-      (sc : FactSet sig) (sc_sub : sc.homSubset fs) (sc_strong : sc.isStrongCore) :
-      sc.modelsKb kb := by
-
-    rcases sc_sub with ⟨sc_sub, h_fs_sc, h_fs_sc_hom⟩
-
-    have h_fs_sc_endo_sc : h_fs_sc.isHomomorphism sc sc := by
-      constructor
-      . exact h_fs_sc_hom.left
-      . apply Set.subset_trans (b := h_fs_sc.applyFactSet fs)
-        . apply TermMapping.apply_generalized_atom_set_subset_of_subset
-          exact sc_sub
-        . exact h_fs_sc_hom.right
-
-    specialize sc_strong h_fs_sc h_fs_sc_endo_sc
-
-    -- TODO: extract this into a general result; check which properties we really need and want here
-    have ex_inv : ∃ (inv : GroundTermMapping sig), (∀ t, t ∈ sc.terms -> (h_fs_sc (inv t)) = t) ∧ inv.isHomomorphism sc sc := by
-      let inv : GroundTermMapping sig := fun t =>
-        have dev := Classical.propDecidable (t ∈ sc.terms)
-        if t_mem : t ∈ sc.terms
-        then
-          Classical.choose (sc_strong.right.right t t_mem)
-        else
-          t
-
-      have inv_id : (∀ t, t ∈ sc.terms -> (h_fs_sc (inv t)) = t) := by
-        intro t t_mem
-        unfold inv
-        simp [t_mem]
-        have spec := Classical.choose_spec (sc_strong.right.right t t_mem)
-        exact spec.right
-      exists inv
-
-      constructor
-      . exact inv_id
-      . constructor
-        . intro c
-          unfold inv
-          cases Classical.em (GroundTerm.const c ∈ sc.terms) with
-          | inr n_mem => simp [n_mem]
-          | inl mem =>
-            simp only [mem, ↓reduceDIte]
-            have spec := Classical.choose_spec (sc_strong.right.right (GroundTerm.const c) mem)
-            apply sc_strong.right.left
-            . exact spec.left
-            . exact mem
-            . rw [spec.right, h_fs_sc_hom.left]
-        . intro f f_mem
-          rcases f_mem with ⟨f', f'_mem, f_eq⟩
-          have strong := sc_strong.left
-          unfold GroundTermMapping.strong at strong
-          apply Classical.byContradiction
-          intro contra
-          apply strong f
-          . intro t t_mem
-            rw [f_eq] at t_mem
-            unfold TermMapping.apply_generalized_atom at t_mem
-            rw [List.mem_map] at t_mem
-            rcases t_mem with ⟨t', t'_mem, t_eq⟩
-            have t'_mem : t' ∈ sc.terms := by exists f'
-            have spec := Classical.choose_spec (sc_strong.right.right t' t'_mem)
-            rw [← t_eq]
-            unfold inv
-            simp [t'_mem]
-            exact spec.left
-          . exact contra
-          . rw [f_eq]
-            unfold GroundTermMapping.applyFact
-            rw [← TermMapping.apply_generalized_atom_compose']
-            have : TermMapping.apply_generalized_atom (h_fs_sc ∘ inv) f' = f' := by
-              apply TermMapping.apply_generalized_atom_eq_self_of_id_on_terms
-              intro t t_mem
-              rw [Function.comp_apply, inv_id]
-              exists f'
-            rw [this]
-            exact f'_mem
-    rcases ex_inv with ⟨inv, inv_id, inv_hom⟩
-
-    constructor
-    . intro f f_mem
-      have : h_fs_sc.applyFact f = f := by
-        have prop := kb.db.toFactSet.property.right
-        unfold FactSet.isFunctionFree at prop
-        unfold Fact.isFunctionFree at prop
-        specialize prop f f_mem
-        apply TermMapping.apply_generalized_atom_eq_self_of_id_on_terms
-        intro t t_mem
-        rcases (prop t t_mem) with ⟨c, t_eq⟩
-        rw [t_eq]
-        exact h_fs_sc_hom.left
-      rw [← this]
-      apply h_fs_sc_hom.right
-      apply TermMapping.apply_generalized_atom_mem_apply_generalized_atom_set
-      apply fs_model.left
-      exact f_mem
-    . intro r r_mem
-      intro subs loaded
-
-      have fs_models_rule := fs_model.right r r_mem (inv ∘ subs)
-      specialize fs_models_rule (by
-        apply Set.subset_trans (b := inv.applyFactSet sc)
-        . intro f f_mem
-          unfold GroundSubstitution.apply_function_free_conj at f_mem
-          unfold TermMapping.apply_generalized_atom_list at f_mem
-          rw [List.mem_toSet, List.mem_map] at f_mem
-          rcases f_mem with ⟨a, a_mem, f_eq⟩
-          rw [← GroundSubstitution.apply_function_free_atom.eq_def, GroundSubstitution.apply_function_free_atom_compose_of_isIdOnConstants _ _ inv_hom.left] at f_eq
-          rw [← f_eq]
-          apply TermMapping.apply_generalized_atom_mem_apply_generalized_atom_set
-          apply loaded
-          unfold GroundSubstitution.apply_function_free_conj
-          unfold TermMapping.apply_generalized_atom_list
-          rw [List.mem_toSet, List.mem_map]
-          exists a
-        . apply Set.subset_trans (b := sc)
-          . exact inv_hom.right
-          . exact sc_sub
-      )
-      rcases fs_models_rule with ⟨i, subs', frontier_mapping, sub_mapping⟩
-
-      exists i
-      exists (h_fs_sc ∘ subs')
-      constructor
-      . intro v v_mem
-        rw [Function.comp_apply]
-        rw [frontier_mapping v v_mem]
-        rw [Function.comp_apply]
-        rw [inv_id _ (by
-          unfold Rule.frontier at v_mem
-          rw [List.mem_filter] at v_mem
-          have v_mem := v_mem.left
-          unfold FunctionFreeConjunction.vars at v_mem
-          rw [List.mem_flatMap] at v_mem
-          rcases v_mem with ⟨a, a_mem, v_mem⟩
-          exists subs.apply_function_free_atom a
+          exists VarOrConst.var v
           constructor
-          . apply loaded
-            unfold GroundSubstitution.apply_function_free_conj
-            unfold TermMapping.apply_generalized_atom_list
-            rw [List.mem_toSet, List.mem_map]
-            exists a
-          . unfold GroundSubstitution.apply_function_free_atom
-            unfold TermMapping.apply_generalized_atom
-            rw [List.mem_map]
-            exists VarOrConst.var v
-            constructor
-            . unfold FunctionFreeAtom.variables at v_mem
-              apply VarOrConst.filterVars_occur_in_original_list
-              exact v_mem
-            . rfl
-        )]
-      . apply Set.subset_trans (b := h_fs_sc.applyFactSet fs)
-        . intro f f_mem
-          unfold GroundSubstitution.apply_function_free_conj at f_mem
-          unfold TermMapping.apply_generalized_atom_list at f_mem
-          rw [List.mem_toSet, List.mem_map] at f_mem
-          rcases f_mem with ⟨a, a_mem, f_eq⟩
-          rw [← GroundSubstitution.apply_function_free_atom.eq_def, GroundSubstitution.apply_function_free_atom_compose_of_isIdOnConstants _ _ h_fs_sc_hom.left] at f_eq
-          rw [← f_eq]
-          apply TermMapping.apply_generalized_atom_mem_apply_generalized_atom_set
-          apply sub_mapping
-          unfold GroundSubstitution.apply_function_free_conj
-          unfold TermMapping.apply_generalized_atom_list
-          rw [List.mem_toSet, List.mem_map]
-          exists a
-        . exact h_fs_sc_hom.right
+          . unfold FunctionFreeAtom.variables at v_mem
+            apply VarOrConst.filterVars_occur_in_original_list
+            exact v_mem
+          . rfl
+      )]
+    . apply Set.subset_trans (b := h_fs_sc.applyFactSet fs)
+      . intro f f_mem
+        unfold GroundSubstitution.apply_function_free_conj at f_mem
+        unfold TermMapping.apply_generalized_atom_list at f_mem
+        rw [List.mem_toSet, List.mem_map] at f_mem
+        rcases f_mem with ⟨a, a_mem, f_eq⟩
+        rw [← GroundSubstitution.apply_function_free_atom.eq_def, GroundSubstitution.apply_function_free_atom_compose_of_isIdOnConstants _ _ h_fs_sc_hom.left] at f_eq
+        rw [← f_eq]
+        apply TermMapping.apply_generalized_atom_mem_apply_generalized_atom_set
+        apply sub_mapping
+        unfold GroundSubstitution.apply_function_free_conj
+        unfold TermMapping.apply_generalized_atom_list
+        rw [List.mem_toSet, List.mem_map]
+        exists a
+      . exact h_fs_sc_hom.right
 
-  theorem strong_core_of_universal_model_is_universal_model
-      {kb : KnowledgeBase sig}
-      (fs : FactSet sig) (fs_univ_model : fs.universallyModelsKb kb)
-      (sc : FactSet sig) (sc_sub : sc.homSubset fs) (sc_strong : sc.isStrongCore) :
-      sc.universallyModelsKb kb := by
+/-- Building on top of the previous theorem, a strong core of a universal model is not only a model but also universal. -/
+theorem strong_core_of_universal_model_is_universal_model
+    {kb : KnowledgeBase sig}
+    (fs : FactSet sig) (fs_univ_model : fs.universallyModelsKb kb)
+    (sc : FactSet sig) (sc_sub : sc.homSubset fs) (sc_strong : sc.isStrongCore) :
+    sc.universallyModelsKb kb := by
+  constructor
+  . exact strong_core_of_model_is_model fs fs_univ_model.left sc sc_sub sc_strong
+  . intro m m_model
+    rcases fs_univ_model.right m m_model with ⟨h, h_hom⟩
+    exists h
     constructor
-    . exact strong_core_of_model_is_model fs fs_univ_model.left sc sc_sub sc_strong
-    . intro m m_model
-      rcases fs_univ_model.right m m_model with ⟨h, h_hom⟩
-      exists h
-      constructor
-      . exact h_hom.left
-      . apply Set.subset_trans (b := h.applyFactSet fs)
-        . apply TermMapping.apply_generalized_atom_set_subset_of_subset
-          exact sc_sub.left
-        . exact h_hom.right
+    . exact h_hom.left
+    . apply Set.subset_trans (b := h.applyFactSet fs)
+      . apply TermMapping.apply_generalized_atom_set_subset_of_subset
+        exact sc_sub.left
+      . exact h_hom.right
 
 end FactSet
 
