ExistentialRules/Models/Basic.lean
@@ -1,29 +1,41 @@
 import ExistentialRules.AtomsAndFacts.Basic
 import ExistentialRules.AtomsAndFacts.SubstitutionsAndHomomorphisms
 
+/-!
+# Models
+
+`FactSet`s can model rules, databases and knowledge bases in a first order logic sense.
+Here, we briefly define what this formally means in terms of our definitions.
+-/
+
 namespace FactSet
 
-  variable {sig : Signature} [DecidableEq sig.P] [DecidableEq sig.C] [DecidableEq sig.V]
+variable {sig : Signature} [DecidableEq sig.P] [DecidableEq sig.C] [DecidableEq sig.V]
 
-  def modelsDb (fs : FactSet sig) (db : Database sig) : Prop :=
-    db.toFactSet.val ⊆ fs
+/-- A `FactSet` models a `Database` if the database is a subset of the fact set. -/
+def modelsDb (fs : FactSet sig) (db : Database sig) : Prop :=
+  db.toFactSet.val ⊆ fs
 
-  def modelsRule (fs : FactSet sig) (rule : Rule sig) : Prop :=
-    ∀ (s : GroundSubstitution sig),
-      ((s.apply_function_free_conj rule.body).toSet ⊆ fs) ->
-        ∃ (i : Fin rule.head.length) (s' : GroundSubstitution sig),
-          (∀ v, v ∈ rule.frontier → s' v = s v) ∧
-          ((s'.apply_function_free_conj (rule.head.get i)).toSet ⊆ fs)
+/-- A `FactSet` models a `Rule` if each substitution that matches the rule body in the fact set can be existended to a substitution for some head of the rule such that this mapped head is already contained in the fact set. The extension of the substitution intuitivly tries to find a suitable mapping for the existential variables that show that the rule is already satisfied (under FOL semantics). -/
+def modelsRule (fs : FactSet sig) (rule : Rule sig) : Prop :=
+  ∀ (s : GroundSubstitution sig),
+    ((s.apply_function_free_conj rule.body).toSet ⊆ fs) ->
+      ∃ (i : Fin rule.head.length) (s' : GroundSubstitution sig),
+        (∀ v, v ∈ rule.frontier → s' v = s v) ∧
+        ((s'.apply_function_free_conj (rule.head.get i)).toSet ⊆ fs)
 
-  def modelsRules (fs : FactSet sig) (rules : RuleSet sig) : Prop :=
-    ∀ r, r ∈ rules.rules -> fs.modelsRule r
+/-- A `FactSet` models a `RuleSet` if it models each rule. -/
+def modelsRules (fs : FactSet sig) (rules : RuleSet sig) : Prop :=
+  ∀ r, r ∈ rules.rules -> fs.modelsRule r
 
-  def modelsKb (fs : FactSet sig) (kb : KnowledgeBase sig) : Prop :=
-    fs.modelsDb kb.db ∧ fs.modelsRules kb.rules
+/-- A `FactSet` models a `KnowledgeBase` if it models both the database and the rule set. -/
+def modelsKb (fs : FactSet sig) (kb : KnowledgeBase sig) : Prop :=
+  fs.modelsDb kb.db ∧ fs.modelsRules kb.rules
 
-  def universallyModelsKb (fs : FactSet sig) (kb : KnowledgeBase sig) : Prop :=
-    fs.modelsKb kb ∧
-    (∀ (m : FactSet sig), m.modelsKb kb -> ∃ (h : GroundTermMapping sig), h.isHomomorphism fs m)
+/-- A `FactSet` $F$ universally models a `KnowledgeBase` if it models the knowledge base but also, for each model $M$ of the knowledge base, we can find a homomorphism from $F$ into $M$. Intuitively, universal models are the *most general* models (but not necessarily the smallest ones). -/
+def universallyModelsKb (fs : FactSet sig) (kb : KnowledgeBase sig) : Prop :=
+  fs.modelsKb kb ∧
+  (∀ (m : FactSet sig), m.modelsKb kb -> ∃ (h : GroundTermMapping sig), h.isHomomorphism fs m)
 
 end FactSet
 
